finish erasure of IO instrumentation

channel.v
@@ -7,35 +7,6 @@ From iris Require Import proofmode.tactics.
 From iris.program_logic Require Import weakestpre lifting.
 From iris.algebra Require Import agree frac.
 
-CoInductive interleaving {A} : Stream A → Stream A → Stream A → Prop :=
-  interL v μ1 μ2 μ : interleaving μ1 μ2 μ →
-                     interleaving {|Shead := v; Stail := μ1 |} μ2
-                                  {|Shead := v; Stail := μ |}
-| interR v μ1 μ2 μ : interleaving μ1 μ2 μ →
-                     interleaving μ1 {|Shead := v; Stail := μ2 |}
-                                  {|Shead := v; Stail := μ |}.
-
-Lemma interleaving_inh {A} (μ1 μ2 : Stream A) : (interleaving μ1 μ2) μ1.
-Proof.
-  revert μ1 μ2.
-  cofix.
-  destruct μ1.
-  by constructor.
-Qed.
-
-Fixpoint append_l_s {A} (l : list A) (s : Stream A) :=
-  match l with
-  | [] => s
-  | a :: l' => {|Shead := a; Stail := append_l_s l' s |}
-  end.
-
-Lemma append_l_s_app {A} (vs : list A) v μ :
-  append_l_s (vs ++ [v]) μ = append_l_s vs {| Shead := v; Stail := μ |}.
-Proof.
-  induction vs; simpl; first done.
-  by rewrite IHvs.
-Qed.
-
 Class ChannelIG Σ := channelIG {
    stream_inG :> inG Σ (prodR (fracR) (agreeR (leibnizC (Stream val))));
    streams_inG :> inG Σ (prodR (fracR) (agreeR (leibnizC ((Stream val) → Prop))))
@@ -430,6 +401,3 @@ Section channels.
   Qed.
 
 End channels.
-
-
-
