full_erasure.v
@@ -1,0 +1,133 @@
+From iris.program_logic Require Export language ectx_language ectxi_language.
+From iris_io.prelude Require Export base.
+From iris_io Require Export proph_erasure lang_proph_erased
+     lang_fully_erased.
+From stdpp Require Import gmap.
+
+Require Import Coq.Logic.FunctionalExtensionality.
+Require Import Coq.Logic.PropExtensionality.
+Require Import Coq.Logic.Classical.
+
+Definition prefix_closed (M : ioSpec) :=
+  ∀ τ τ', M (τ ++ τ') → M τ.
+
+Definition IO_performed
+           (σ : language.state PE_lang) (σ' : language.state PFE_lang) M
+  := (EHeap σ) = (FEHeap σ') ∧ (EProph σ) = (FEProph σ') ∧
+     (EioState σ) = (λ τ, M ((FEIO σ') ++ τ)) ∧ (∃ τ, M ((FEIO σ') ++ τ)).
+
+Definition make_ioSpec (σ : language.state PFE_lang) M :
+  language.state PE_lang :=
+  {| EHeap := FEHeap σ; EProph := FEProph σ;
+     EioState := λ τ, M ((FEIO σ) ++ τ) |}.
+
+Lemma make_ioSpec_IO_performed σ (M : ioSpec):
+  M (FEIO σ) → IO_performed (make_ioSpec σ M) σ M.
+Proof.
+  destruct σ as [h p i]; repeat split; simpl in *; eauto.
+  by eexists nil; rewrite app_nil_r.
+Qed.
+
+Lemma fully_erased_reachable_reachable th1 h1 th2 σ2 (M : ioSpec) :
+  prefix_closed M →
+  M (FEIO σ2) →
+  rtc (@step PFE_lang) (th1, {| FEHeap := h1; FEProph := ∅; FEIO := [] |})
+      (th2, σ2) →
+  rtc (@step PE_lang)
+      (th1, {| EHeap := h1; EProph := ∅; EioState := M |})
+      (th2, make_ioSpec σ2 M).
+Proof.
+  intros Mpc.
+  remember (th1, {| FEHeap := h1; FEProph := ∅; FEIO := [] |}) as cfg.
+  remember (th2, σ2) as cfg'.
+  intros HM Hrtc; revert HM.
+  revert th1 h1 th2 σ2 Heqcfg Heqcfg'.
+  simpl in *.
+  eapply (rtc_ind_r_weak
+            (λ z z', ∀ (th1 : list (language.expr PFE_lang))
+                       (h1 : gmap loc val)
+                       (th2 : list (language.expr PFE_lang))
+                       (σ2 : language.state PFE_lang),
+                z = (th1,
+                     {| FEHeap := h1; FEProph := ∅; FEIO := [] |})
+                → z' = (th2, σ2) →
+                M (FEIO σ2) →
+                rtc (@step PE_lang)
+                    (th1, {| EHeap := h1; EProph := ∅; EioState := M |})
+                    (th2, make_ioSpec σ2 M)));
+    last eauto.
+  - intros x th1 h1 th2 σ2 Heqcfg Heqcfg'; simplify_eq.
+    left; split; simpl; eauto; econstructor.
+  - intros x y z Hxy Hyz IH th1 h1 th2 σ2 Heqcfg Heqcfg' HM;
+      simplify_eq; simpl in *.
+    destruct y as [yh yp].
+    inversion Hyz as [? ? ? ? ? ? ? ? ? Hpr]; simplify_eq.
+    inversion Hpr as [? ? ? ? ? Hestp]; simpl in *; simplify_eq.
+    inversion Hestp; simplify_eq;
+      repeat match goal with
+      | H : is_Some _ |- _ => destruct H
+      end;
+      try (by eapply rtc_r; first (by apply IH); repeat econstructor; eauto).
+    eapply rtc_r; first apply IH; eauto.
+    + simpl in HM; eapply Mpc; eauto.
+    + unfold make_ioSpec; simpl.
+      replace (λ τ, M ((FEIO σ1 ++ [(t, v, v')]) ++ τ)) with
+        (λ τ, M (FEIO σ1 ++ [(t, v, v')] ++ τ)); last first.
+    { extensionality τ. by rewrite -assoc. }
+    repeat econstructor; eauto; simpl.
+    apply (EIOS t e v v' {| EioState := λ τ, M (FEIO σ1 ++ τ) |}); eauto.
+Qed.
+
+Definition fully_erased_safe e (M : ioSpec) :=
+  ∀ th2 σ2,
+    M (FEIO σ2) →
+    rtc (@step PFE_lang) ([e], {| FEHeap := ∅; FEProph := ∅; FEIO := [] |})
+        (th2, σ2) →
+    ∀ e, e ∈ th2 → AsVal e ∨
+                   (∃ e' σ'' efs,
+                       @language.prim_step PFE_lang e σ2 e' σ'' efs
+                       ∧ ∀ t v v', FEIO σ'' = FEIO σ2 ++ [(t, v, v')] →
+                                   ∃ v'', M (FEIO σ2 ++ [(t, v, v'')])).
+
+Lemma reducible_fully_erase_reducible e σ σ' M :
+  IO_performed σ σ' M →
+  @language.reducible PE_lang e σ →
+  ∃ e' σ'' efs,
+    @language.prim_step PFE_lang e σ' e' σ'' efs
+    ∧ ∀ t v v', FEIO σ'' = FEIO σ' ++ [(t, v, v')] →
+                ∃ v'', M (FEIO σ' ++ [(t, v, v'')]).
+Proof.
+  intros Hsp (e'&σ2&efs&Hrd); simpl in *.
+  inversion Hrd as [K e1' e2' ? ? Hhrd]; simpl in *; subst.
+  destruct σ as [σh σp]; destruct σ' as [σ'h σ'p];
+    destruct Hsp as [? [? [? ?]]]; simpl in *; simplify_eq.
+  inversion Hhrd; subst;
+    repeat match goal with A : is_Some _ |- _ => destruct A as [? ?] end;
+    simpl in *;
+    try (by (unshelve (repeat econstructor; eauto)); simpl in *;
+            try match goal with
+                | H : ?A = ?A ++ [_] |- _ =>
+                  let H' := fresh in
+                  pose proof (f_equal length H) as H';
+                  rewrite app_length in H'; simpl in H'; omega
+                end).
+  - eexists _, _, _; split; first by unshelve (repeat econstructor; eauto).
+    intros ? ? ? ?; simpl in *;
+      match goal with
+      | H: ?A ++ [_] = ?A ++ [_] |- _ =>
+        apply app_inv_head in H; simplify_eq; simpl in *; eauto
+      end.
+Qed.
+
+Lemma soundness_prophecies e M :
+  prefix_closed M → erased_safe e M → fully_erased_safe e M.
+Proof.
+  intros Hpc Hs th2 σ2 HMσ2 Hrtc re Hre.
+  assert (rtc (@language.step PE_lang)
+              ([e], {| EHeap := ∅; EProph := ∅; EioState := M |})
+              (th2, make_ioSpec σ2 M)) as Hrtc'.
+  { eapply fully_erased_reachable_reachable; eauto. }
+  edestruct Hs as [?|Hred]; eauto.
+  right. eapply reducible_fully_erase_reducible; eauto.
+  by apply make_ioSpec_IO_performed.
+Qed.
