lang_fully_erased.v
@@ -1,0 +1,136 @@
+From iris.program_logic Require Export language ectx_language ectxi_language.
+From iris_io.prelude Require Export base.
+From iris_io Require Export lang_proph_erased.
+From iris.algebra Require Export ofe.
+From stdpp Require Import gmap.
+
+Module Plang_fully_erased.
+
+  Record fully_erased_state : Type :=
+    { FEHeap : gmap loc val;
+      FEProph : (gset loc);
+      FEIO : list (ioTag * val * val)
+    }.
+
+  Definition update_FEheap σ h :=
+    {| FEHeap := h; FEProph := FEProph σ; FEIO := FEIO σ |}.
+
+  Definition update_FEproph σ ι :=
+    {| FEHeap := FEHeap σ; FEProph := ι; FEIO := FEIO σ |}.
+
+   Definition update_FEIO σ τ :=
+    {| FEHeap := FEHeap σ; FEProph := FEProph σ; FEIO := τ |}.
+
+  Inductive fully_erased_head_step :
+    expr → fully_erased_state → expr → fully_erased_state → list expr → Prop :=
+  (* β *)
+  | FEBetaS e1 e2 v2 σ :
+      to_val e2 = Some v2 →
+      fully_erased_head_step (App (Rec e1) e2) σ e1.[(Rec e1), e2/] σ []
+  | FEZetaS e1 e2 v1 σ :
+      to_val e1 = Some v1 →
+      fully_erased_head_step (LetIn e1 e2) σ e2.[e1/] σ []
+  | FELamBetaS e1 e2 v2 σ :
+      to_val e2 = Some v2 →
+      fully_erased_head_step (App (Lam e1) e2) σ e1.[e2/] σ []
+  | FESeqS e1 e2 v1 σ :
+      to_val e1 = Some v1 →
+      fully_erased_head_step (Seq e1 e2) σ e2 σ []
+  (* Products *)
+  | FEFstS e1 v1 e2 v2 σ :
+      to_val e1 = Some v1 → to_val e2 = Some v2 →
+      fully_erased_head_step (Fst (Pair e1 e2)) σ e1 σ []
+  | FESndS e1 v1 e2 v2 σ :
+      to_val e1 = Some v1 → to_val e2 = Some v2 →
+      fully_erased_head_step (Snd (Pair e1 e2)) σ e2 σ []
+  (* Sums *)
+  | FECaseLS e0 v0 e1 e2 σ :
+      to_val e0 = Some v0 →
+      fully_erased_head_step (Case (InjL e0) e1 e2) σ e1.[e0/] σ []
+  | FECaseRS e0 v0 e1 e2 σ :
+      to_val e0 = Some v0 →
+      fully_erased_head_step (Case (InjR e0) e1 e2) σ e2.[e0/] σ []
+    (* nat bin op *)
+  | FEBinOpS op a b σ :
+      fully_erased_head_step (BinOp op (#n a) (#n b)) σ (of_val (binop_eval op a b)) σ []
+  (* If then else *)
+  | FEIfFalse e1 e2 σ :
+      fully_erased_head_step (If (#♭ false) e1 e2) σ e2 σ []
+  | FEIfTrue e1 e2 σ :
+      fully_erased_head_step (If (#♭ true) e1 e2) σ e1 σ []
+  (* Recursive Types *)
+  | FEUnfold_Fold e v σ :
+      to_val e = Some v →
+      fully_erased_head_step (Unfold (Fold e)) σ e σ []
+  (* Polymorphic Types *)
+  | FETBeta e σ :
+      fully_erased_head_step (TApp (TLam e)) σ e σ []
+  (* Concurrency *)
+  | FEForkS e σ:
+      fully_erased_head_step (Fork e) σ Unit σ [e]
+  (* Reference Types *)
+  | FEAllocS e v σ l :
+     to_val e = Some v → (FEHeap σ) !! l = None →
+     fully_erased_head_step (Alloc e) σ (Loc l) (update_FEheap σ (<[l:=v]>(FEHeap σ))) []
+  | FELoadS l v σ :
+     (FEHeap σ) !! l = Some v →
+     fully_erased_head_step (Load (Loc l)) σ (of_val v) σ []
+  | FEStoreS l e v σ :
+     to_val e = Some v → is_Some ((FEHeap σ) !! l) →
+     fully_erased_head_step (Store (Loc l) e) σ Unit (update_FEheap σ (<[l:=v]>(FEHeap σ))) []
+  (* Compare and swap *)
+  | FECasFailS l e1 v1 e2 v2 vl σ :
+     to_val e1 = Some v1 → to_val e2 = Some v2 →
+     (FEHeap σ) !! l = Some vl → vl ≠ v1 →
+     fully_erased_head_step (CAS (Loc l) e1 e2) σ (#♭ false) σ []
+  | FECasSucS l e1 v1 e2 v2 σ :
+     to_val e1 = Some v1 → to_val e2 = Some v2 →
+     (FEHeap σ) !! l = Some v1 →
+     fully_erased_head_step (CAS (Loc l) e1 e2) σ (#♭ true) (update_FEheap σ (<[l:=v2]>(FEHeap σ))) []
+  (* Prophecy operational semantics *)
+  | FECreate_PrS σ :
+      fully_erased_head_step Create_Pr σ (Pr (fresh (FEProph σ)))
+                       (update_FEproph σ ({[fresh (FEProph σ)]} ∪ (FEProph σ))) []
+  | FEAssignS v l e σ :
+     l ∈ (FEProph σ) → to_val e = Some v →
+     fully_erased_head_step (Assign_Pr (Pr l) e) σ Unit σ []
+  | FERandS b σ : fully_erased_head_step Rand σ (Bool b) σ []
+  | FEIOS t e v v' σ : to_val e = Some v →
+                    fully_erased_head_step (IO t e) σ (of_val v')
+                              (update_FEIO σ ((FEIO σ) ++ [(t, v, v')])) [].
+
+  (** Basic properties about the language *)
+  Lemma val_stuck e1 σ1 e2 σ2 ef :
+    fully_erased_head_step e1 σ1 e2 σ2 ef → to_val e1 = None.
+  Proof. destruct 1; naive_solver. Qed.
+
+  Lemma head_ctx_step_val Ki e σ1 e2 σ2 ef :
+    fully_erased_head_step (fill_item Ki e) σ1 e2 σ2 ef → is_Some (to_val e).
+  Proof. destruct Ki; inversion_clear 1; simplify_option_eq; eauto. Qed.
+
+  Lemma alloc_fresh e v σ :
+    let l := fresh (dom (gset loc) (FEHeap σ)) in
+    to_val e = Some v → fully_erased_head_step (Alloc e) σ (Loc l)
+                                         (update_FEheap σ (<[l:=v]>(FEHeap σ))) [].
+  Proof. by intros; apply FEAllocS, (not_elem_of_dom (D:=gset loc)), is_fresh. Qed.
+
+  Lemma val_head_stuck e1 σ1 e2 σ2 efs : fully_erased_head_step e1 σ1 e2 σ2 efs → to_val e1 = None.
+  Proof. destruct 1; naive_solver. Qed.
+
+  Lemma lang_mixin : EctxiLanguageMixin of_val to_val fill_item
+                                        fully_erased_head_step.
+  Proof.
+    split; apply _ || eauto using to_of_val, of_to_val, val_head_stuck,
+           fill_item_val, fill_item_no_val_inj, head_ctx_step_val.
+  Qed.
+
+End Plang_fully_erased.
+
+Canonical Structure PFE_ectxi_lang :=
+  EctxiLanguage Plang_fully_erased.lang_mixin.
+Canonical Structure PFE_ectx_lang :=
+  EctxLanguageOfEctxi PFE_ectxi_lang.
+Canonical Structure PFE_lang :=
+  LanguageOfEctx PFE_ectx_lang.
+
+Export Plang_fully_erased.
